more CDCL

Weidenbach_Book/Propo_CDCL2.thy
@@ -5,7 +5,6 @@ begin
 
 type_synonym ('v, 'lvl, 'mark) cdcl_state = "('v, 'lvl, 'mark) annoted_lits \<times> 'v clauses"
 
-
 inductive propagate :: "('v, 'lvl, 'mark) cdcl_state \<Rightarrow> ('v, 'lvl, 'mark) cdcl_state \<Rightarrow> bool" where
 propagate[intro]: "C + {#L#} \<in> N \<Longrightarrow> M \<Turnstile>as CNot C \<Longrightarrow> undefined_lit L M \<Longrightarrow> propagate (M, N) ((Propagated L mark) # M, N)"
 
@@ -105,8 +104,10 @@ lemma cdcl_sat_iff:
   shows "I \<Turnstile>s N \<longleftrightarrow> I \<Turnstile>s N'"
   using assms apply (induction rule: cdcl_all_induct)
      using dpll_sat_iff apply blast
-    unfolding true_clss_cls_def total_over_m_def apply (metis atms_of_m_singleton atms_of_m_union sup.orderE true_clss_insert)
-  unfolding true_clss_insert atms_of_m_singleton atms_of_m_union by (metis atms_of_m_insert insert_Diff total_over_set_union true_clss_insert)
+    unfolding true_clss_cls_def total_over_m_def apply (metis atms_of_m_singleton atms_of_m_union 
+      sup.orderE true_clss_insert)
+  unfolding true_clss_insert atms_of_m_singleton atms_of_m_union by (metis atms_of_m_insert 
+    insert_Diff total_over_set_union true_clss_insert)
 
 
 lemma dpll_atms_of_m_clauses_inv:
@@ -117,7 +118,8 @@ lemma dpll_atms_of_m_clauses_inv:
 lemma dpll_atms_of_m_clauses_decreasing:
   assumes "cdcl (M, N) (M', N')"
   shows "atms_of_m N' \<subseteq> atms_of_m N"
-  using assms by (induction rule: cdcl_all_induct) (auto dest!: dpll_atms_of_m_clauses_inv simp add: atms_of_m_def)
+  using assms by (induction rule: cdcl_all_induct) 
+    (auto dest!: dpll_atms_of_m_clauses_inv simp add: atms_of_m_def)
 
 lemma dpll_atms_in_trail:
   assumes "dpll (M, N) (M', N')"
@@ -138,7 +140,7 @@ lemma cdcl_atms_in_trail:
   shows "atm_of ` (lits_of M') \<subseteq> atms_of_m N"
   using assms
   by (induction rule: cdcl_all_induct)
-    (simp_all add: dpll_atms_in_trail dpll_atms_of_m_clauses_inv)
+     (simp_all add: dpll_atms_in_trail dpll_atms_of_m_clauses_inv)
 
 
 lemma cdcl_atms_in_trail_in_set:
@@ -148,15 +150,17 @@ lemma cdcl_atms_in_trail_in_set:
   shows "atm_of ` (lits_of M') \<subseteq> A"
   using assms
   by (induction rule: cdcl_all_induct)
-    (simp_all add: dpll_atms_in_trail_in_set dpll_atms_of_m_clauses_inv)
+     (simp_all add: dpll_atms_in_trail_in_set dpll_atms_of_m_clauses_inv)
 
 subsection \<open>Measure\<close>
 
 subsection\<open>Adding the measure based on Nieuwenhuis et al.\<close>
-abbreviation latm ::  "'a list \<Rightarrow> 'b literal multiset set \<Rightarrow> nat" where
-  "latm M N \<equiv> card (atms_of_m N) - length M"
+text \<open>The idea is to measure the \<^emph>\<open>progress\<close> of the proof: we are measuring how many literals are 
+  unassigned, either locally (between two decisions) or globally.\<close>
+abbreviation unassigned_lit ::  "'a list \<Rightarrow> 'b literal multiset set \<Rightarrow> nat" where
+  "unassigned_lit M N \<equiv> card (atms_of_m N) - length M"
 
-abbreviation "trail_mes_l N M M' \<equiv> ((\<exists>M''. M = M' @ M'' \<and> latm M N < latm M' N))"
+abbreviation "trail_mes_l N M M' \<equiv> ((\<exists>M''. M = M' @ M'' \<and> unassigned_lit M N < unassigned_lit M' N))"
 
 abbreviation "full_trail_mes N M M' \<equiv> (trail_mes_l N M M' \<or> trail_mes_l N M' M)"
 
@@ -217,27 +221,26 @@ abbreviation all_bounded_list_different :: "nat \<Rightarrow> nat \<Rightarrow> 
   {((T, u), (S, y)). ((length S < p \<and> (\<forall>n \<in> set S. n < m)) \<and> (length T < p \<and> (\<forall>n \<in> set T. n < m)))
      \<and> \<not>(\<exists>S'. T = S @ S') \<and> (T, S) \<in> lexord less_than}"
 
-abbreviation fst_same_beginning_snd_decreasing :: "(('a list \<times> nat) \<times> 'a list \<times> nat) set" where
-"fst_same_beginning_snd_decreasing  \<equiv> {((a, b),(c, d)). b < d \<and> (\<exists>l. a = c @ l)}"
+abbreviation fst_same_beginning_snd_decreasing :: 
+  "nat \<Rightarrow> 'c \<Rightarrow> (('c :: ord list \<times> nat) \<times> 'c ::ord list \<times> nat) set" where
+"fst_same_beginning_snd_decreasing \<equiv> (\<lambda>p m. 
+  {((a, b),(c, d)). ((length a < p \<and> (\<forall>n \<in> set a. n < m)) \<and> (length c < p \<and> (\<forall>n \<in> set c. n < m)))
+     \<and> b < d \<and> (\<exists>l. a = c @ l)})"
 
 
 lemma wf_bounded_distinct_different_lexord:
-  "wf(all_bounded_list_different m p)"
+  "wf (all_bounded_list_different m p)"
   apply (rule wf_fst_wf_pair)
-  by (rule wf_subset[OF wf_bounded_distinct_lexord])
-     (auto intro: wf_bounded_distinct_lexord)
+  by (rule wf_subset[OF wf_bounded_distinct_lexord]) auto
 
 lemma wf_trail_mes_l_bounded:
   assumes H: "\<And>M. P M \<Longrightarrow> distinct M \<and> set M \<subseteq> A"
   shows "wf {(M', M). trail_mes_l A M' M \<and> P M \<and> P M'}"
-  by (insert wf_measure[of "\<lambda>M. latm M A"])
+  by (insert wf_measure[of "\<lambda>M. unassigned_lit M A"])
      (auto dest!: assms intro: wf_subset simp add: measure_def inv_image_def less_than_def less_eq)
-(* definition lexord_d :: "(nat list \<times> nat list) set" where
-"lexord_d = lexord less_than \<inter> {((M', N'), (M, N)). \<not>(\<exists>T. M = M' @ T)}"
- *)
 
 lemma wf_fst_same_beginning_snd_decreasing:
-  "wf fst_same_beginning_snd_decreasing"
+  "wf (fst_same_beginning_snd_decreasing p m)"
 proof -
   have "wf {((a, b::nat),(c, d)). b < d}"
     by (rule wf_snd_wf_pair) (rule Wellfounded.wf_less)
@@ -245,16 +248,18 @@ proof -
     by (rule wf_subset) auto
 qed
 
-lemma "wf (all_bounded_list_different p m \<union> fst_same_beginning_snd_decreasing)"
-       apply (rule wf_Un[OF wf_bounded_distinct_different_lexord wf_fst_same_beginning_snd_decreasing])
-       apply simp
-       apply auto
- oops
+lemma fst_same_beginning_snd_decreasing_all_bounded_list_different_disj:
+  "fst_same_beginning_snd_decreasing r s \<inter> all_bounded_list_different m p = {}"
+  by auto
 
+lemma "wf (all_bounded_list_different n p \<union> fst_same_beginning_snd_decreasing r s)" (is "wf (?B\<union>?F)")
+apply (rule wf_union_compatible[OF wf_bounded_distinct_different_lexord wf_fst_same_beginning_snd_decreasing])
+apply simp
+oops
 
 fun trail_mes ::  "'v literal multiset set \<Rightarrow> ('v, 'lvl, 'mark) cdcl_state \<Rightarrow> nat list" where
 "trail_mes A (M, N) =
-  (map (\<lambda>(_, propa). latm propa A) (rev (get_all_marked_decomposition M)))"
+  (map (\<lambda>(_, propa). unassigned_lit propa A) (rev (get_all_marked_decomposition M)))"
 
 lemma length_get_all_marked_decomposition_append_Marked:
   "length (get_all_marked_decomposition (F' @ Marked K d # F)) =
@@ -265,9 +270,9 @@ lemma length_get_all_marked_decomposition_append_Marked:
 
 lemma take_length_get_all_marked_decomposition_marked_sandwich:
   "take (length (get_all_marked_decomposition F))
-      (map (\<lambda>(_, propa). latm propa A) (rev (get_all_marked_decomposition (F' @ Marked K d # F))))
+      (map (\<lambda>(_, propa). unassigned_lit propa A) (rev (get_all_marked_decomposition (F' @ Marked K d # F))))
       =
-     map (\<lambda>(_, propa). latm propa A) (rev (get_all_marked_decomposition F))
+     map (\<lambda>(_, propa). unassigned_lit propa A) (rev (get_all_marked_decomposition F))
     "
 proof (induction F' rule: marked_lit_list_induct)
   case nil
@@ -290,7 +295,7 @@ lemma length_get_all_marked_decomposition_length:
   "length (get_all_marked_decomposition M) \<le> 1 + length M"
   by (induction M rule: marked_lit_list_induct) auto
 
-lemma tl_get_all_marked__append_marked_not_nil:
+lemma tl_get_all_marked_append_marked_not_nil:
   "tl (get_all_marked_decomposition (xs @ [Marked K d])) \<noteq> []"
   by (induction xs rule: marked_lit_list_induct) auto
 
@@ -298,22 +303,22 @@ lemma last_tl_get_all_marked_decomposition_propagated_tl:
   "last (tl (get_all_marked_decomposition (xs @ [Marked K d]))) =
     last (get_all_marked_decomposition (xs @ [Marked K d]))"
   by (induction xs rule: marked_lit_list_induct)
-     (simp_all add: tl_get_all_marked__append_marked_not_nil)
+     (simp_all add: tl_get_all_marked_append_marked_not_nil)
 
 lemma last_get_all_marked_decomposition_propagated_empty:
   "last (get_all_marked_decomposition (xs @ [Marked K d])) = ([], [])"
   by (induction xs rule: marked_lit_list_induct)
-     (auto simp add: tl_get_all_marked__append_marked_not_nil
+     (auto simp add: tl_get_all_marked_append_marked_not_nil
        last_tl_get_all_marked_decomposition_propagated_tl)
 
 lemma "tl (map snd (butlast (get_all_marked_decomposition (xs @ [Marked K d]))))
   = map snd (butlast (tl (get_all_marked_decomposition (xs @ [Marked K d])))) "
   by (cases "get_all_marked_decomposition (xs @ [Marked K d])") auto
 
-lemma [simp]: "butlast (get_all_marked_decomposition (F' @ [Marked K d])) \<noteq> []"
-    by (metis append_Nil get_all_marked_decomposition_never_empty list.sel(3) snoc_eq_iff_butlast
-      tl_get_all_marked__append_marked_not_nil)
-
+lemma butlast_get_all_marked_decomposition_append_marked[simp]:
+  "butlast (get_all_marked_decomposition (F' @ [Marked K d])) \<noteq> []"
+  by (metis append_Nil get_all_marked_decomposition_never_empty list.sel(3) snoc_eq_iff_butlast
+    tl_get_all_marked_append_marked_not_nil)
 
 
 lemma map_snd_get_all_marked_decomposition_marked:
@@ -332,19 +337,24 @@ next
     by (cases "get_all_marked_decomposition (F' @ [Marked K d])") auto
   have [simp]: "snd (hd (get_all_marked_decomposition (F' @ Marked K d # F)))
     = snd (hd (get_all_marked_decomposition (F' @ [Marked K d])))"
-    by (smt append_butlast_last_id append_is_Nil_conv append_self_conv2 get_all_marked_decomposition_never_empty hd_append list.collapse list.inject list.map_sel(1) proped.IH tl_get_all_marked__append_marked_not_nil)
+    by (smt append_butlast_last_id append_is_Nil_conv append_self_conv2 get_all_marked_decomposition_never_empty hd_append list.collapse list.inject list.map_sel(1) proped.IH tl_get_all_marked_append_marked_not_nil)
 
   obtain a b l where F: "get_all_marked_decomposition (F' @ Marked K d # F) = (a, b) # l"
     by (cases "get_all_marked_decomposition (F' @ Marked K d # F)") auto
   thus ?case unfolding F
-    by (auto simp add: map_tl tl_get_all_marked__append_marked_not_nil IH arg_cong[OF IH, of tl] tl_append
+    by (auto simp add: map_tl tl_get_all_marked_append_marked_not_nil IH arg_cong[OF IH, of tl] tl_append
     dest!: arg_cong[of "_#_" _ hd] split: list.split)
 qed
 
-lemma map_latm_pair_map_latm_map_snd:
-  "map (\<lambda>(_, propa). latm propa A) l = map (\<lambda>p. latm p A) (map snd l)"
+lemma map_unassigned_lit_pair_map_unassigned_lit_map_snd:
+  "map (\<lambda>(_, propa). unassigned_lit propa A) l = map (\<lambda>p. unassigned_lit p A) (map snd l)"
  by (fastforce simp: o_def )
 
+text \<open>The upper bound is @{term "card (atms_of_m A)+2"}:
+  \<^item> @{term "card (atms_of_m A)"} is the total number of atoms
+  \<^item> @{term "1"} comes the fact that the bound in @{term all_bounded_list_different} is strict
+  \<^item> the second @{term 1} is here for technical reasons: @{term get_all_marked_decomposition} can 
+  generate an empty couple at the end of the list.\<close>
 lemma dpll_trail_mes_decreasing':
   fixes M :: "('v, 'lvl, 'mark) annoted_lits " and N :: "'v clauses"
   assumes "dpll (M, N) (M', N')" and
@@ -352,9 +362,9 @@ lemma dpll_trail_mes_decreasing':
   "atm_of ` lits_of M \<subseteq> atms_of_m A" and
   "no_dup M" and
   finite: "finite A"
-  shows "((trail_mes A (M', N'), latm M' A), (trail_mes A (M, N), latm M A))
+  shows "((trail_mes A (M', N'), unassigned_lit M' A), (trail_mes A (M, N), unassigned_lit M A))
      \<in> all_bounded_list_different (card (atms_of_m A)+2) (card (atms_of_m A)+2)
-       \<union> fst_same_beginning_snd_decreasing"
+       \<union> fst_same_beginning_snd_decreasing (card (atms_of_m A)+2) (card (atms_of_m A)+2)"
   using assms
 proof (induction rule: dpll_all_induct)
   case (propagate C L N M d) note CLN = this(1) and MC =this(2) and undef_L = this(3) and A = this(4) and MA = this(5)
@@ -374,12 +384,12 @@ proof (induction rule: dpll_all_induct)
   hence l: "length (Propagated L d # M) \<le>  card (atms_of_m A)"
     using incl finite unfolding distinctlength_eq_card_atm_of_lits_of[OF no_dup]
     by (simp add: card_mono)
-  hence latm: "latm b A = Suc (latm (Propagated L d # b) A)"
+  hence unassigned_lit: "unassigned_lit b A = Suc (unassigned_lit (Propagated L d # b) A)"
     using b_le_M by force
-  moreover have "length l < Suc (card (atms_of_m A))"
+  moreover have "length l < card (atms_of_m A)"
     using length_get_all_marked_decomposition_length[of M] l unfolding M by auto
   ultimately show ?case using no_dup l
-    by (auto simp: lexord_def lex_conv latm M)
+    by (auto simp: lexord_def lex_conv unassigned_lit M)
 next
   case (decide L M N lv) note undef_L = this(1) and MC =this(2) and NA = this(3) and A = this(4) and MA = this(5)
   have "atms_of_m N' \<subseteq> atms_of_m A"
@@ -398,11 +408,14 @@ next
   hence l: "length (Marked L lv # M) \<le>  card (atms_of_m A)"
     using incl finite unfolding distinctlength_eq_card_atm_of_lits_of[OF no_dup]
     by (simp add: card_mono)
-  hence latm: "latm M A = Suc (latm (Marked L lv # M) A)"
+  hence unassigned_lit: "unassigned_lit M A = Suc (unassigned_lit (Marked L lv # M) A)"
     using b_le_M by force
-  show ?case by (auto simp add: latm)
+  moreover have "length (get_all_marked_decomposition M) < Suc (card (atms_of_m A))"
+    using length_get_all_marked_decomposition_length[of M] l by auto
+  ultimately show ?case using l by (auto simp add: unassigned_lit)
 next
-  case (backjump C N F' K d F L _ lv) note undef_L = this(1) and MC =this(2) and NA = this(3) and A = this(4) and MA = this(5) and nd = this(8)
+  case (backjump C N F' K d F L _ lv) note undef_L = this(1) and MC =this(2) and NA = this(3) and
+    A = this(4) and MA = this(5) and nd = this(8)
   have "atms_of_m N' \<subseteq> atms_of_m A"
     using assms(1) assms(2) dpll_atms_of_m_clauses_inv by blast
   have incl: "atm_of ` lits_of (Propagated L lv # F) \<subseteq> atms_of_m A"
@@ -416,45 +429,46 @@ next
     using get_all_marked_decomposition_decomp[of M] by (simp add: M)
   have "finite (atms_of_m A)" using finite by simp
 
-  hence F_le_A: "length (Propagated L lv # F) \<le>  card (atms_of_m A)"
-    using incl finite unfolding distinctlength_eq_card_atm_of_lits_of[OF no_dup]
+  hence F_le_A: "length (Propagated L lv # F) \<le> card (atms_of_m A)"
+    using incl unfolding distinctlength_eq_card_atm_of_lits_of[OF no_dup]
     by (simp add: card_mono)
 
   obtain a b l where F: "get_all_marked_decomposition F = (a, b) # l"
     by (cases "get_all_marked_decomposition F") auto
 
   hence "F = b @ a"
-    using get_all_marked_decomposition_decomp[of "Propagated L lv # F" a "Propagated L lv # b"] by simp
-  hence latm: "latm b A = Suc (latm (Propagated L lv # b) A)"
-     using F_le_A by simp
+    using get_all_marked_decomposition_decomp[of "Propagated L lv # F" a "Propagated L lv # b"] 
+    by simp
+  hence unassigned_lit: "unassigned_lit b A = Suc (unassigned_lit (Propagated L lv # b) A)"
+    using F_le_A by simp
   have l_F: "length (F' @ Marked K d # F) \<le> card (atms_of_m A)"
-    by (metis `finite (atms_of_m A)` backjump.prems(2) card_mono distinctlength_eq_card_atm_of_lits_of nd)
-  hence l_g_a: "length (get_all_marked_decomposition (F' @ Marked K d # F)) < Suc (Suc (card (atms_of_m A)))"
+    by (metis `finite (atms_of_m A)` backjump.prems(2) distinctlength_eq_card_atm_of_lits_of nd
+      card_mono)
+  hence l_g_a: "length (get_all_marked_decomposition (F' @ Marked K d # F)) 
+    < Suc (Suc (card (atms_of_m A)))"
     using length_get_all_marked_decomposition_length[of "F' @ Marked K d # F"] by auto
 
-  have length_l_A: "length l <  (card (atms_of_m A))"
-    using length_get_all_marked_decomposition_length[of F] unfolding F
-    by (metis F_le_A Groups.add_ac(2) Nat.le_trans One_nat_def Suc_le_lessD
-      add.right_neutral add_Suc_right list.size(4))
+  have length_l_A: "Suc (length l) <  1 + card (atms_of_m A)"
+    using length_get_all_marked_decomposition_length[of F]  F_le_A unfolding F by auto
   show ?case
     proof (cases F')
       case Nil
-      have "((trail_mes A (Propagated L lv # F, N), latm (Propagated L lv # F) A), trail_mes A (F' @ Marked K d # F, N), latm (F' @ Marked K d # F) A)
+      have "((trail_mes A (Propagated L lv # F, N), unassigned_lit (Propagated L lv # F) A), trail_mes A (F' @ Marked K d # F, N), unassigned_lit (F' @ Marked K d # F) A)
     \<in> all_bounded_list_different (card (atms_of_m A) + 2) (card (atms_of_m A) + 2)"
-        using length_l_A by (auto simp add: F latm Nil lexord_def)
+        using length_l_A by (auto simp add: F unassigned_lit Nil lexord_def)
       thus ?thesis by simp
     next
       case (Cons f F'') note F' = this(1)
-      have R: "rev (map (\<lambda>(_, propa). latm propa A) (get_all_marked_decomposition (F' @ Marked K d # F))) =
-        rev (map (\<lambda>p. latm p A) (map snd (butlast (get_all_marked_decomposition (F' @ [Marked K d])) @ get_all_marked_decomposition F)))"
-        unfolding map_latm_pair_map_latm_map_snd map_snd_get_all_marked_decomposition_marked
-        by (auto simp: F latm)
-      have "((trail_mes A (Propagated L lv # F, N), latm (Propagated L lv # F) A), trail_mes A (F' @ Marked K d # F, N), latm (F' @ Marked K d # F) A)
+      have R: "rev (map (\<lambda>(_, propa). unassigned_lit propa A) (get_all_marked_decomposition (F' @ Marked K d # F))) =
+        rev (map (\<lambda>p. unassigned_lit p A) (map snd (butlast (get_all_marked_decomposition (F' @ [Marked K d])) @ get_all_marked_decomposition F)))"
+        unfolding map_unassigned_lit_pair_map_unassigned_lit_map_snd map_snd_get_all_marked_decomposition_marked
+        by (auto simp: F unassigned_lit)
+      have "((trail_mes A (Propagated L lv # F, N), unassigned_lit (Propagated L lv # F) A), trail_mes A (F' @ Marked K d # F, N), unassigned_lit (F' @ Marked K d # F) A)
               \<in> all_bounded_list_different (card (atms_of_m A) + 2) (card (atms_of_m A) + 2)"
               (* TODO: Improve proof *)
         using l_F l_g_a length_l_A apply (auto simp add: F rev_map[symmetric])
-        unfolding map_latm_pair_map_latm_map_snd map_snd_get_all_marked_decomposition_marked
-        by (auto simp: F latm lexord_def)
+        unfolding map_unassigned_lit_pair_map_unassigned_lit_map_snd map_snd_get_all_marked_decomposition_marked
+        by (auto simp: F unassigned_lit lexord_def)
       thus ?thesis by simp
     qed
 qed
